more

tarjan.v
@@ -566,6 +566,17 @@ let fold u strict accu :=
 in
 UMap.fold fold ltle (UMap.empty bool, false).
 
+Record clean_ltle_Spec g (m1 m2 : UMap.t bool) (chg : bool) : Prop := {
+  cltle_l : forall u b, UMap.MapsTo u m1 b -> exists v, UMap.MapsTo v m2 b /\ Rel.eq g u v;
+  cltle_r : forall u b, UMap.MapsTo u m2 b -> exists v, UMap.MapsTo v m1 b /\ Rel.eq g u v;
+  cltle_u : forall u v, UMap.In u m1 -> UMap.In v m2 -> Rel.eq g u v -> Level.eq u v;
+  cltle_b : if chg then True else UMap.Equal m1 m2
+}.
+
+Lemma clean_ltle_spec : forall (g : Universes) ltle
+  (m : forall u, UMap.In u ltle -> UMap.In u g.(entries)),
+  let '(ans, chg) := clean_ltle g ltle m in clean_ltle_Spec g.(entries) ltle ans chg.
+
 Lemma clean_ltle_identity : forall (g : Universes) ltle
   (m : forall u, UMap.In u ltle -> UMap.In u g.(entries)),
   let ans := clean_ltle g ltle m in
